stackLang definition complete

new-backend/word_lang/stackLangScript.sml
@@ -20,7 +20,7 @@ val _ = Datatype `
              | Set store_name ('a word_exp)
              | Call ((stack_prog # num # num) option)
                     (* return var, return-handler code, labels l1,l2*)
-                    (num option) (* target of call *)
+                    (num + num) (* target of call *)
                     ((stack_prog # num # num) option)
                     (* handler: exception-handler code, labels l1,l2*)
              | Seq stack_prog stack_prog
@@ -39,16 +39,17 @@ val _ = Datatype `
 
 val _ = Datatype `
   stack_state =
-    <| locals  : ('a word_loc) num_map
+    <| regs  : ('a word_loc) num_map
      ; store   : store_name |-> 'a word_loc
      ; stack   : ('a word_loc) list
+     ; stack_shadow : ('a word_loc) list
      ; memory  : 'a word -> 'a word_loc
      ; mdomain : ('a word) set
      ; permute : num -> num -> num (* sequence of bijective mappings *)
      ; gc_fun  : 'a gc_fun_type
      ; handler : num (*position of current handle frame on stack*)
      ; clock   : num
-     ; code    : (num # ('a word_prog) # num) num_map
+     ; code    : ('a stack_prog) num_map
      ; output  : string |> `
 
 val mem_store_def = Define `
@@ -90,7 +91,7 @@ val MEM_IMP_word_exp_size = store_thm("MEM_IMP_word_exp_size",
 val word_exp_def = tDefine "word_exp" `
   (word_exp s (Const w) = SOME w) /\
   (word_exp s (Var v) =
-     case lookup v s.locals of
+     case lookup v s.regs of
      | SOME (Word w) => SOME w
      | _ => NONE) /\
   (word_exp s (Lookup name) =
@@ -125,7 +126,7 @@ val isException_def = Define `
   (isException (Exception a b) = T) /\ (isException _ = F)`;
 
 val get_var_def = Define `
-  get_var v (s:'a stack_state) = sptree$lookup v s.locals`;
+  get_var v (s:'a stack_state) = sptree$lookup v s.regs`;
 
 val get_vars_def = Define `
   (get_vars [] s = SOME []) /\
@@ -143,11 +144,11 @@ val list_insert_def = Define `
 
 val set_var_def = Define `
   set_var v x (s:'a stack_state) =
-    (s with locals := (insert v x s.locals))`;
+    (s with regs := (insert v x s.regs))`;
 
 val set_vars_def = Define `
   set_vars vs xs (s:'a stack_state) =
-    (s with locals := (list_insert vs xs s.locals))`;
+    (s with regs := (list_insert vs xs s.regs))`;
 
 val set_store_def = Define `
   set_store v x (s:'a stack_state) = (s with store := s.store |+ (v,x))`;
@@ -160,6 +161,10 @@ val check_clock_thm = prove(
   ``(check_clock s1 s2).clock <= s2.clock /\
     (s1.clock <= s2.clock ==> (check_clock s1 s2 = s1))``,
   SRW_TAC [] [check_clock_def])
+
+val check_clock_alt = prove(
+  ``(s1.clock <= (dec_clock s2).clock ==> (check_clock s1 s2 = s1))``,
+  SRW_TAC [] [check_clock_def,dec_clock_def] \\ `F` by DECIDE_TAC)
 
 val check_clock_lemma = prove(
   ``b ==> ((check_clock s1 s).clock < s.clock \/
@@ -186,123 +191,17 @@ val EVEN_fromList2 = store_thm("EVEN_fromList2",
     |> SIMP_RULE (srw_ss()) [GSYM fromList2_def]
     |> GEN_ALL) \\ fs []);
 
-val call_env_def = Define `
-  call_env args (s:'a word_state) =
-    s with <| locals := fromList2 args |>`;
-
-val list_rearrange_def = Define `
-  list_rearrange mover xs =
-    (* if the mover function is actually a permutation,
-     i.e. it bijects (or injects) the keys 0...n-1 to 0...n-1
-     use it *)
-    if (BIJ mover (count (LENGTH xs)) (count (LENGTH xs))) then
-      GENLIST (\i. EL (mover i) xs) (LENGTH xs)
-    else (* if it isn't well-formed, just pretend it is I *)
-      xs`
-
-(* Compare on keys, if keys match (never), then compare on
-   the word_loc vals. Treat Words as < Locs *)
-val key_val_compare_def = Define `
-  key_val_compare x y =
-    let (a:num,b) = x in
-    let (a':num,b') = y in
-      (a < a') \/
-      (a = a' /\
-        case b of
-          Word x => (case b' of Word y => x <= y | _ => T)
-        | Loc a b => case b' of Loc a' b' => (a<a') \/ (a=a' /\ b<=b') | _ => F)`
-
-(*
-EVAL ``key_val_compare (1,Loc 3 4) (1,Loc 1 2)``
-*)
-
-val env_to_list_def = Define `
-  env_to_list env (bij_seq:num->num->num) =
-    let mover = bij_seq 0 in
-    let permute = (\n. bij_seq (n + 1)) in
-    let l = toAList env in
-    let l = QSORT key_val_compare l in
-    let l = list_rearrange mover l in
-      (l,permute)`
-
-val push_env_def = Define `
-  (push_env env NONE s =
-    let (l,permute) = env_to_list env s.permute in
-      s with <| stack := StackFrame l NONE :: s.stack
-              ; permute := permute|>) ∧
-  (push_env env (SOME (w:num,h:'a word_prog,l1,l2)) s =
-    let (l,permute) = env_to_list env s.permute in
-      let handler = SOME (s.handler,l1,l2) in
-      s with <| stack := StackFrame l handler :: s.stack
-              ; permute := permute
-              ; handler := LENGTH s.stack|>)`;
-
-val pop_env_def = Define `
-  pop_env s =
-    case s.stack of
-    | (StackFrame e NONE::xs) =>
-         SOME (s with <| locals := fromAList e ; stack := xs |>)
-    | (StackFrame e (SOME (n,_,_))::xs) =>
-         SOME (s with <| locals := fromAList e ; stack := xs ; handler := n |>)
-    | _ => NONE`;
+val empty_env_def = Define `
+  empty_env (s:'a stack_state) = s with <| regs := LN ; stack := [] |>`;
 
 val jump_exc_def = Define `
   jump_exc s =
     if s.handler < LENGTH s.stack then
       case LAST_N (s.handler+1) s.stack of
-      | StackFrame e (SOME (n,l1,l2)) :: xs =>
-          SOME (s with <| handler := n ; locals := fromAList e ; stack := xs |>,l1,l2)
+      | Word _ :: Loc l1 l2 :: Word w :: xs =>
+          SOME (s with <| handler := w2n w ; stack := xs |>,l1,l2)
       | _ => NONE
     else NONE`;
-
-val cut_env_def = Define `
-  cut_env (name_set:num_set) env =
-    if domain name_set SUBSET domain env
-    then SOME (inter env name_set)
-    else NONE`
-
-val cut_state_def = Define `
-  cut_state names s =
-    case cut_env names s.locals of
-    | NONE => NONE
-    | SOME env => SOME (s with locals := env)`;
-
-val cut_state_opt_def = Define `
-  cut_state_opt names s =
-    case names of
-    | NONE => SOME s
-    | SOME names => cut_state names s`;
-
-val pop_env_clock = prove(
-  ``(pop_env s = SOME s1) ==> (s1.clock = s.clock)``,
-  fs [pop_env_def]
-  \\ REPEAT BasicProvers.FULL_CASE_TAC \\ fs []
-  \\ SRW_TAC [] [] \\ fs []);
-
-val push_env_clock = prove(
-  ``(push_env env b s).clock = s.clock``,
-  Cases_on `b` \\ TRY(PairCases_on`x`) \\ fs [push_env_def]
-  \\ REPEAT BasicProvers.FULL_CASE_TAC \\ fs []
-  \\ SRW_TAC [] [] \\ fs []);
-
-val find_code_def = Define `
-  (find_code (SOME p) args code =
-     case sptree$lookup p code of
-     | NONE => NONE
-     | SOME (_,exp,arity) => if LENGTH args = arity then SOME (args,exp)
-                                                    else NONE) /\
-  (find_code NONE args code =
-     if args = [] then NONE else
-       case LAST args of
-       | Loc loc 0 =>
-           (case lookup loc code of
-            | NONE => NONE
-            | SOME (_,exp,arity) => if LENGTH args = arity + 1
-                                    then SOME (FRONT args,exp)
-                                    else NONE)
-       | other => NONE)`
-
-
 
 val bit_length_def = Define `
   bit_length w = if w = 0w then 0 else bit_length (w >>> 1) + 1`;
@@ -395,8 +294,8 @@ val dec_stack_def = Define `
            | NONE => NONE
            | SOME ws3 => SOME (w1 ++ ws1 ++ ws3))`
 
-val wGC_def = Define `  (* wGC runs the garbage collector algorithm *)
-  wGC s =
+val sGC_def = Define `  (* wGC runs the garbage collector algorithm *)
+  sGC s =
     case enc_stack s.stack of
     | NONE => NONE
     | SOME wl_list =>
@@ -410,28 +309,18 @@ val wGC_def = Define `  (* wGC runs the garbage collector algorithm *)
                           ; store := st
                           ; memory := m |>))`
 
-
-
 val has_space_def = Define `
-  has_space wl s =
+  has_space wl (s:'a stack_state) =
     case (wl, FLOOKUP s.store NextFree, FLOOKUP s.store LastFree) of
     | (Word w, SOME (Word n), SOME (Word l)) => SOME (w2n w <= w2n (l - n))
     | _ => NONE`
 
-val wAlloc_def = Define `
-  wAlloc (w:'a word) names s =
-    (* prune local names *)
-    case cut_env names s.locals of
-    | NONE => (SOME Error,s)
-    | SOME env =>
-     (* perform garbage collection *)
-     (case wGC (push_env env (NONE:(num # 'a word_prog # num # num) option) (set_store AllocSize (Word w) s)) of
+val sAlloc_def = Define `
+  sAlloc (w:'a word) (s:'a stack_state) =
+    (* perform garbage collection *)
+      case sGC (set_store AllocSize (Word w) s) of
       | NONE => (SOME Error,s)
       | SOME s =>
-       (* restore local variables *)
-       (case pop_env s of
-        | NONE => (SOME Error, s)
-        | SOME s =>
          (* read how much space should be allocated *)
          (case FLOOKUP s.store AllocSize of
           | NONE => (SOME Error, s)
@@ -442,7 +331,7 @@ val wAlloc_def = Define `
             | SOME T => (* success there is that much space *)
                         (NONE,s)
             | SOME F => (* fail, GC didn't free up enough space *)
-                        (SOME NotEnoughSpace,call_env [] s with stack:= [])))))`
+                        (SOME NotEnoughSpace,empty_env s)))`
 
 val word_assign_def = Define `
   word_assign reg exp s =
@@ -451,7 +340,7 @@ val word_assign_def = Define `
      | SOME w => SOME (set_var reg (Word w) s)`;
 
 val wInst_def = Define `
-  wInst i s =
+  wInst i (s:'a stack_state) =
     case i of
     | Skip => SOME s
     | Const reg w => word_assign reg (Const w) s
@@ -474,129 +363,108 @@ val wInst_def = Define `
     | _ => NONE`
 
 val get_var_imm_def = Define`
-  (get_var_imm ((Reg n):'a reg_imm) s = get_var n s) ∧
+  (get_var_imm ((Reg n):'a reg_imm) s = get_var n s) /\
   (get_var_imm (Imm w) s = SOME(Word w))`
 
+val find_code_def = Define `
+  (find_code (INL p) regs code = sptree$lookup p code) /\
+  (find_code (INR r) regs code =
+     case lookup r regs of
+       SOME (Loc loc 0) => lookup loc code
+     | other => NONE)`
 
-
-val wEval_def = tDefine "wEval" `
-  (wEval (Skip:'a word_prog,s) = (NONE,s:'a word_state)) /\
-  (wEval (Alloc n names,s) =
+val sEval_def = tDefine "sEval" `
+  (sEval (Skip:'a stack_prog,s) = (NONE,s:'a stack_state)) /\
+  (sEval (Alloc n,s) =
      case get_var n s of
-     | SOME (Word w) => wAlloc w names s
+     | SOME (Word w) => sAlloc w s
      | _ => (SOME Error,s)) /\
-  (wEval (Move pri moves,s) =
-     if ALL_DISTINCT (MAP FST moves) then
-       case get_vars (MAP SND moves) s of
-       | NONE => (SOME Error,s)
-       | SOME vs => (NONE, set_vars (MAP FST moves) vs s)
-     else (SOME Error,s)) /\
-  (wEval (Inst i,s) =
+  (sEval (Inst i,s) =
      case wInst i s of
      | SOME s1 => (NONE, s1)
      | NONE => (SOME Error, s)) /\
-  (wEval (Assign v exp,s) =
-     case word_exp s exp of
-     | NONE => (SOME Error, s)
-     | SOME w => (NONE, set_var v (Word w) s)) /\
-  (wEval (Get v name,s) =
+  (sEval (Get v name,s) =
      case FLOOKUP s.store name of
      | NONE => (SOME Error, s)
      | SOME x => (NONE, set_var v x s)) /\
-  (wEval (Set v exp,s) =
+  (sEval (Set v exp,s) =
      case word_exp s exp of
      | NONE => (SOME Error, s)
      | SOME w => (NONE, set_store v (Word w) s)) /\
-  (wEval (Store exp v,s) =
-     case (word_exp s exp, get_var v s) of
-     | (SOME a, SOME w) =>
-         (case mem_store a w s of
-          | SOME s1 => (NONE, s1)
-          | NONE => (SOME Error, s))
-     | _ => (SOME Error, s)) /\
-  (wEval (Tick,s) =
-     if s.clock = 0 then (SOME TimeOut,call_env [] s with stack := [])
+  (sEval (Tick,s) =
+     if s.clock = 0 then (SOME TimeOut,empty_env s)
                     else (NONE,dec_clock s)) /\
-  (wEval (Seq c1 c2,s) =
-     let (res,s1) = wEval (c1,s) in
-       if res = NONE then wEval (c2,check_clock s1 s) else (res,s1)) /\
-  (wEval (Return n m,s) =
+  (sEval (Seq c1 c2,s) =
+     let (res,s1) = sEval (c1,s) in
+       if res = NONE then sEval (c2,check_clock s1 s) else (res,s1)) /\
+  (sEval (Return n m,s) =
      case (get_var n s ,get_var m s) of
-     | (SOME x,SOME y) => (SOME (Result x y),call_env [] s)
+     | (SOME x,SOME y) => (SOME (Result x y),empty_env s)
      | _ => (SOME Error,s)) /\
-  (wEval (Raise n,s) =
+  (sEval (Raise n,s) =
      case get_var n s of
      | NONE => (SOME Error,s)
      | SOME w =>
        (case jump_exc s of
         | NONE => (SOME Error,s)
         | SOME (s,l1,l2) => (SOME (Exception (Loc l1 l2) w)),s)) /\
-  (wEval (If cmp r1 ri c1 c2,s) =
+  (sEval (If cmp r1 ri c1 c2,s) =
     (case (get_var r1 s,get_var_imm ri s)of
     | SOME (Word x),SOME (Word y) =>
-      if word_cmp cmp x y then wEval (c1,s)
-                          else wEval (c2,s)
+      if word_cmp cmp x y then sEval (c1,s)
+                          else sEval (c2,s)
     | _ => (SOME Error,s))) /\
-  (wEval (Call ret dest args handler,s) =
-     case get_vars args s of
+  (sEval (Call ret dest handler,s) =
+     case find_code dest s.regs s.code of
      | NONE => (SOME Error,s)
-     | SOME xs =>
-       (case find_code dest xs s.code of
-	  | NONE => (SOME Error,s)
-	  | SOME (args1,prog) =>
-	    (case ret of
-	     | NONE (* tail call *) =>
-	       if handler = NONE then
-           if s.clock = 0 then (SOME TimeOut,call_env [] s with stack := []) else
-           (case wEval (prog, call_env args1 (dec_clock s)) of
-            | (NONE,s) => (SOME Error,s)
-            | (SOME res,s) => (SOME res,s))
-               else (SOME Error,s)
-	     | SOME (n,names,ret_handler,l1,l2) (* returning call, returns into var n *) =>
-	       (case cut_env names s.locals of
-		| NONE => (SOME Error,s)
-		| SOME env =>
-	       if s.clock = 0 then (SOME TimeOut,call_env [] s with stack := []) else
-	       (case wEval (prog, call_env ((Loc l1 l2)::args1)
-		       (push_env env handler (dec_clock s))) of
-		| (SOME (Result x y),s2) =>
-      if x ≠ Loc l1 l2 then (SOME Error,s2)
-      else
-		   (case pop_env s2 of
-		    | NONE => (SOME Error,s2)
-		    | SOME s1 =>
-			(if domain s1.locals = domain env
-			 then
-			   (*Value restriction on the return handler (makes it easier to reason about)
-			     Don't really need it to do fancy things.
-           Keep y in register 2
-           *)
-			   case wEval(ret_handler,set_var n y (check_clock s1 s)) of
-			   | (NONE,s) => (NONE,s)
-			   | (_,s) => (SOME Error,s)
-			 else (SOME Error,s1)))
-		| (SOME (Exception x y),s2) =>
-		   (case handler of (* if handler is present, then handle exc *)
-		    | NONE => (SOME (Exception x y),s2)
-		    | SOME (n,h,l1,l2) =>
-        if x ≠ Loc l1 l2 then (SOME Error,s2)
-        else
-          (if domain s2.locals = domain env
-           then wEval (h, set_var n y (check_clock s2 s))
-           else (SOME Error,s2)))
-        | (NONE,s) => (SOME Error,s)
-		| res => res))))) `
- (WF_REL_TAC `(inv_image (measure I LEX measure (word_prog_size (K 0)))
-                            (\(xs,(s:'a word_state)). (s.clock,xs)))`
+     | SOME prog =>
+     case ret of
+     (* tail call *)
+     | NONE =>
+        if handler <> NONE then (SOME Error,s) else
+        if s.clock = 0 then (SOME TimeOut,empty_env s) else
+          (case sEval (prog,dec_clock s) of
+           | (NONE,s) => (SOME Error,s)
+           | (SOME res,s) => (SOME res,s))
+     (* returning call, returns into var n *)
+     | SOME (ret_handler,l1,l2) =>
+        if s.clock = 0 then (SOME TimeOut,empty_env s) else
+          (case sEval (prog, dec_clock s) of
+           | (SOME (Result x y),s2) =>
+               if x <> Loc l1 l2 then (SOME Error,s2) else
+                 (case sEval(ret_handler,check_clock s2 s) of
+                  | (NONE,s) => (NONE,s)
+                  | (_,s) => (SOME Error,s))
+           | (SOME (Exception x y),s2) =>
+               (case handler of (* if handler is present, then handle exc *)
+                | NONE => (SOME (Exception x y),s2)
+                | SOME (h,l1,l2) =>
+                   if x <> Loc l1 l2 then (SOME Error,s2) else
+                     sEval (h, check_clock s2 s))
+           | (NONE,s) => (SOME Error,s)
+           | res => res)) /\
+  (sEval (StackAlloc n,s) =
+     if LENGTH s.stack_shadow < n then (SOME NotEnoughSpace,empty_env s) else
+       (NONE, s with <| stack := TAKE n s.stack_shadow ++ s.stack ;
+                        stack_shadow := DROP n s.stack_shadow |>)) /\
+  (sEval (StackFree n,s) =
+     if LENGTH s.stack < n then (SOME Error,empty_env s) else
+       (NONE, s with <| stack := DROP n s.stack ;
+                        stack_shadow := TAKE n s.stack ++ s.stack_shadow |>)) /\
+  (sEval (StackLoad r n,s) =
+     if LENGTH s.stack < n then (SOME Error,empty_env s) else
+       (NONE, set_var r (EL n s.stack) s)) /\
+  (sEval (StackStore r n,s) =
+     if LENGTH s.stack < n then (SOME Error,empty_env s) else
+       case get_var r s of
+       | NONE => (SOME Error,empty_env s)
+       | SOME v => (NONE, s with stack := LUPDATE v n s.stack))`
+ (WF_REL_TAC `(inv_image (measure I LEX measure (stack_prog_size (K 0)))
+                            (\(xs,(s:'a stack_state)). (s.clock,xs)))`
   \\ REPEAT STRIP_TAC \\ TRY DECIDE_TAC
   \\ TRY (MATCH_MP_TAC check_clock_lemma \\ DECIDE_TAC)
-  \\ TRY
-    (fs[push_env_clock,call_env_def,dec_clock_def]\\DECIDE_TAC)
-  \\ EVAL_TAC
-   \\ Cases_on `s.clock <= s1.clock`
- \\ FULL_SIMP_TAC (srw_ss()) [push_env_clock]
-  \\ IMP_RES_TAC pop_env_clock \\ fs [] \\ SRW_TAC [] []
-  \\ Cases_on `s2.clock < s.clock` \\ fs [] \\ DECIDE_TAC)
+  \\ fs[empty_env_def,dec_clock_def] \\ DECIDE_TAC)
+
 
 (* We prove that the clock never increases. *)
 
@@ -604,35 +472,24 @@ val check_clock_IMP = prove(
   ``n <= (check_clock r s).clock ==> n <= s.clock``,
   SRW_TAC [] [check_clock_def] \\ DECIDE_TAC);
 
-val wGC_clock = store_thm("wGC_clock",
-  ``!s1 s2. (wGC s1 = SOME s2) ==> s2.clock <= s1.clock``,
-  fs [wGC_def,LET_DEF] \\ SRW_TAC [] []
+val sGC_clock = store_thm("sGC_clock",
+  ``!s1 s2. (sGC s1 = SOME s2) ==> s2.clock <= s1.clock``,
+  fs [sGC_def,LET_DEF] \\ SRW_TAC [] []
   \\ REPEAT (BasicProvers.FULL_CASE_TAC \\ SRW_TAC [] [] \\ fs [])
   \\ SRW_TAC [] [] \\ fs []);
 
-val wAlloc_clock = store_thm("wAlloc_clock",
-  ``!xs s1 vs s2. (wAlloc x names s1 = (vs,s2)) ==> s2.clock <= s1.clock``,
-  SIMP_TAC std_ss [wAlloc_def] \\ REPEAT STRIP_TAC
+val sAlloc_clock = store_thm("sAlloc_clock",
+  ``!xs s1 vs s2. (sAlloc x s1 = (vs,s2)) ==> s2.clock <= s1.clock``,
+  SIMP_TAC std_ss [sAlloc_def] \\ REPEAT STRIP_TAC
   \\ REPEAT BasicProvers.FULL_CASE_TAC \\ SRW_TAC [] [] \\ fs []
   \\ REPEAT BasicProvers.FULL_CASE_TAC \\ SRW_TAC [] [] \\ fs []
   \\ Q.ABBREV_TAC `s3 = set_store AllocSize (Word x) s1`
   \\ `s3.clock=s1.clock` by Q.UNABBREV_TAC`s3`>>fs[set_store_def]
   \\ REPEAT BasicProvers.FULL_CASE_TAC \\ SRW_TAC [] [] \\ fs []
-  >- (IMP_RES_TAC wGC_clock \\
-     fs[push_env_def,LET_THM,env_to_list_def] \\
-     unabbrev_all_tac>>fs[])
-  \\ REPEAT BasicProvers.FULL_CASE_TAC \\ SRW_TAC [] [] \\ fs []
-  \\ POP_ASSUM MP_TAC \\ SRW_TAC [] []
-  \\ IMP_RES_TAC pop_env_clock \\ IMP_RES_TAC wGC_clock
-  \\ fs [push_env_clock,set_store_def] \\ SRW_TAC [] []
-  \\ Cases_on `env_to_list s1.locals s1.permute` \\ fs [LET_DEF]\\rfs[]
-  \\ BasicProvers.EVERY_CASE_TAC
-  \\ fs[call_env_def,fetch "-" "word_state_component_equality"]);
-
-val pop_env_clock = prove(
-  ``(pop_env s = SOME t) ==> (s.clock = t.clock)``,
-  fs [pop_env_def] \\ REPEAT BasicProvers.FULL_CASE_TAC
-  \\ SRW_TAC [] [] \\ fs []);
+  \\ IMP_RES_TAC sGC_clock \\ fs []
+  \\ UNABBREV_ALL_TAC \\ fs []
+  \\ Cases_on `x'''` \\ fs [] \\ SRW_TAC [] []
+  \\ EVAL_TAC \\ decide_tac);
 
 val wInst_clock = prove(
   ``wInst i s = SOME s2 ==> s2.clock <= s.clock``,
@@ -641,36 +498,26 @@ val wInst_clock = prove(
   \\ SRW_TAC [] [set_var_def] \\ fs []
   \\ fs [mem_store_def] \\ SRW_TAC [] []);
 
-val wEval_clock = store_thm("wEval_clock",
-  ``!xs s1 vs s2. (wEval (xs,s1) = (vs,s2)) ==> s2.clock <= s1.clock``,
-  recInduct (fetch "-" "wEval_ind") \\ REPEAT STRIP_TAC
-  \\ POP_ASSUM MP_TAC \\ ONCE_REWRITE_TAC [wEval_def]
+val sEval_clock = store_thm("sEval_clock",
+  ``!xs s1 vs s2. (sEval (xs,s1) = (vs,s2)) ==> s2.clock <= s1.clock``,
+  recInduct (fetch "-" "sEval_ind") \\ REPEAT STRIP_TAC
+  \\ POP_ASSUM MP_TAC \\ ONCE_REWRITE_TAC [sEval_def]
   \\ FULL_SIMP_TAC std_ss [cut_state_opt_def]
   \\ BasicProvers.EVERY_CASE_TAC
-  \\ REPEAT STRIP_TAC \\ SRW_TAC [] [check_clock_def,call_env_def]
+  \\ REPEAT STRIP_TAC \\ SRW_TAC [] [check_clock_def,empty_env_def]
   \\ IMP_RES_TAC wInst_clock
-  \\ fs [call_env_def]
-  \\ RES_TAC \\ IMP_RES_TAC check_clock_IMP
-  \\ FULL_SIMP_TAC std_ss [PULL_FORALL] \\ RES_TAC
-  \\ IMP_RES_TAC check_clock_IMP
-  \\ IMP_RES_TAC wAlloc_clock
-  \\ FULL_SIMP_TAC (srw_ss()) [dec_clock_def,set_var_def,
-       jump_exc_def,get_var_def,push_env_clock,set_vars_def,
-       call_env_def,cut_state_def,set_store_def,mem_store_def]
-  \\ REV_FULL_SIMP_TAC std_ss [] \\ RES_TAC
-  \\ IMP_RES_TAC pop_env_clock
-  \\ TRY DECIDE_TAC
-  \\ SRW_TAC [] []
-  \\ Cases_on `wEval (c1,s)` \\ FULL_SIMP_TAC (srw_ss()) [LET_DEF]
+  \\ IMP_RES_TAC sAlloc_clock
+  \\ fs [set_var_def,set_store_def,dec_clock_def,jump_exc_def]
+  \\ Cases_on `sEval (c1,s)` \\ FULL_SIMP_TAC (srw_ss()) [LET_DEF]
   \\ NTAC 5 ((BasicProvers.EVERY_CASE_TAC)
              \\ FULL_SIMP_TAC (srw_ss()) [] \\ SRW_TAC [] [])
   \\ FULL_SIMP_TAC (srw_ss()) []
   \\ IMP_RES_TAC check_clock_IMP
   \\ RES_TAC \\ DECIDE_TAC);
 
-val wEval_check_clock = prove(
-  ``!xs s1 vs s2. (wEval (xs,s1) = (vs,s2)) ==> (check_clock s2 s1 = s2)``,
-  METIS_TAC [wEval_clock,check_clock_thm]);
+val sEval_check_clock = prove(
+  ``!xs s1 vs s2. (sEval (xs,s1) = (vs,s2)) ==> (check_clock s2 s1 = s2)``,
+  METIS_TAC [sEval_clock,check_clock_thm]);
 
 (* Finally, we remove check_clock from the induction and definition theorems. *)
 
@@ -681,7 +528,7 @@ fun sub f tm = f tm handle HOL_ERR _ =>
   handle HOL_ERR _ => tm
 
 val remove_check_clock = sub (fn tm =>
-  if can (match_term ``check_clock s1 (s2:'a word_state)``) tm
+  if can (match_term ``check_clock s1 (s2:'a stack_state)``) tm
   then tm |> rator |> rand else fail())
 
 val remove_disj = sub (fn tm => if is_disj tm then tm |> rator |> rand else fail())
@@ -690,8 +537,8 @@ val set_var_check_clock = prove(
   ``set_var v x (check_clock s1 s2) = check_clock (set_var v x s1) s2``,
   SIMP_TAC std_ss [set_var_def,check_clock_def] \\ SRW_TAC [] []);
 
-val wEval_ind = save_thm("wEval_ind",let
-  val raw_ind = fetch "-" "wEval_ind"
+val sEval_ind = curry save_thm "sEval_ind" let
+  val raw_ind = fetch "-" "sEval_ind"
   val goal = raw_ind |> concl |> remove_check_clock |> remove_disj
   (* set_goal([],goal) *)
   val ind = prove(goal,
@@ -699,103 +546,36 @@ val wEval_ind = save_thm("wEval_ind",let
     \\ REVERSE (REPEAT STRIP_TAC) \\ ASM_REWRITE_TAC []
     THEN1 (FIRST_X_ASSUM MATCH_MP_TAC
            \\ ASM_REWRITE_TAC [] \\ REPEAT STRIP_TAC
-           \\ IMP_RES_TAC wEval_clock \\ SRW_TAC [] []
-           \\ TRY (`s2.clock <= s.clock` by
-            (fs [call_env_def,dec_clock_def,push_env_clock]
-             \\ IMP_RES_TAC pop_env_clock \\ DECIDE_TAC)
-           \\ `s2 = check_clock s2 s` by fs [check_clock_def])
-           \\ TRY (`s1.clock <= s.clock` by
-             (fs [call_env_def,dec_clock_def,push_env_clock]
-             \\ IMP_RES_TAC pop_env_clock \\ DECIDE_TAC)
-           \\ `s1 = check_clock s1 s` by fs[check_clock_def])
-           \\ POP_ASSUM (fn th => ONCE_REWRITE_TAC [th])
-           \\ FIRST_X_ASSUM MATCH_MP_TAC \\ fs [])
+           \\ IMP_RES_TAC sEval_clock \\ SRW_TAC [] []
+           \\ RES_TAC \\ IMP_RES_TAC check_clock_alt \\ fs [])
     \\ FIRST_X_ASSUM (MATCH_MP_TAC)
     \\ ASM_REWRITE_TAC [] \\ REPEAT STRIP_TAC \\ RES_TAC
     \\ REPEAT (Q.PAT_ASSUM `!x.bbb` (K ALL_TAC))
-    \\ IMP_RES_TAC wEval_clock
-    \\ IMP_RES_TAC (GSYM wEval_clock)
+    \\ IMP_RES_TAC sEval_clock
+    \\ IMP_RES_TAC (GSYM sEval_clock)
     \\ FULL_SIMP_TAC (srw_ss()) [check_clock_thm,GSYM set_var_check_clock])
-  val lemma = EVAL ``bool_to_val F = bool_to_val T``
-  in ind |> SIMP_RULE std_ss [lemma] end);
+  in ind end;
 
-val wEval_def = save_thm("wEval_def",let
-  val tm = fetch "-" "wEval_AUX_def"
-           |> concl |> rand |> dest_abs |> snd |> rand |> rand
-  val tm = ``^tm wEval (x,s)``
-  val rhs = SIMP_CONV std_ss [EVAL ``pair_CASE (x,y) f``] tm |> concl |> rand
-  val goal = ``!x s. wEval (x,s) = ^rhs`` |> remove_check_clock |> remove_disj
+val sEval_def = curry save_thm "sEval_def" let
+  val goal = sEval_def |> concl |> remove_check_clock |> remove_disj
   (* set_goal([],goal) *)
   val def = prove(goal,
-    recInduct wEval_ind
-    \\ REPEAT STRIP_TAC
-    \\ SIMP_TAC (srw_ss()) []
-    \\ TRY (SIMP_TAC std_ss [Once wEval_def] \\ NO_TAC)
-    \\ REPEAT (POP_ASSUM (K ALL_TAC))
-    \\ SIMP_TAC std_ss [Once wEval_def]
-    \\ Cases_on `wEval (c1,s)`
-    \\ Cases_on `wEval (p,s)`
-    \\ Cases_on `wEval (g,s)`
-    \\ FULL_SIMP_TAC (srw_ss()) [LET_DEF]
-    \\ IMP_RES_TAC wEval_check_clock \\ FULL_SIMP_TAC std_ss []
-    \\ REPEAT BasicProvers.CASE_TAC
-    \\ SRW_TAC [] [] \\ IMP_RES_TAC wEval_check_clock
-    \\ FULL_SIMP_TAC (srw_ss()) [check_clock_def]
-    \\ fs [pop_env_def,call_env_def,dec_clock_def,push_env_clock]
-    \\ SRW_TAC [] []
-    \\ IMP_RES_TAC wEval_clock
-    \\ fs [call_env_def,dec_clock_def,push_env_clock]
-    \\ `x''.clock <= s.clock` by
-         (BasicProvers.EVERY_CASE_TAC>>fs[fetch "-" "word_state_component_equality"]>>
-         `F` by DECIDE_TAC) \\ fs[]
-    \\ TRY (`x''.clock = r'''''.clock` by
-       (BasicProvers.EVERY_CASE_TAC>>fs[fetch "-" "word_state_component_equality"]))
-    \\ TRY (`x''.clock = r''''''.clock` by
-       (BasicProvers.EVERY_CASE_TAC>>fs[fetch "-" "word_state_component_equality"]))
-    \\ `F` by DECIDE_TAC)
-  val new_def = wEval_def |> CONJUNCTS |> map (fst o dest_eq o concl o SPEC_ALL)
-                  |> map (REWR_CONV def THENC SIMP_CONV (srw_ss()) [])
-                  |> LIST_CONJ
-  in new_def end);
+    REPEAT STRIP_TAC
+    \\ SIMP_TAC std_ss [Once sEval_def] \\ fs []
+    \\ Cases_on `sEval (c1,s)` \\ fs [LET_DEF]
+    \\ IMP_RES_TAC sEval_check_clock \\ fs []
+    \\ Cases_on `find_code dest s.regs s.code` \\ fs []
+    \\ Cases_on `sEval (x,dec_clock s)` \\ fs []
+    \\ `check_clock r' s = r'` by ALL_TAC \\ fs []
+    \\ IMP_RES_TAC sEval_check_clock
+    \\ fs [check_clock_def,dec_clock_def] \\ SRW_TAC [] []
+    \\ fs [theorem "stack_state_component_equality"]
+    \\ Cases_on `r'.clock <= s.clock - 1` \\ fs []
+    \\ DECIDE_TAC)
+  in def end;
 
 (* clean up *)
 
-val _ = map delete_binding ["wEval_AUX_def", "wEval_primitive_def"];
+val _ = map delete_binding ["sEval_AUX_def", "sEval_primitive_def"];
 
-(*
-
-  BVP --> word_lang compiler correctness thm:
-
-    pEval (prog,s1) = (res,s2) ==>
-    state_rel s1 t1 ==>
-      wEval (pCompile prog,t1) = (res1,t2) /\
-      state_rel s2 t2 /\ res_rel res res1
-
-  word_lang --> word_lang compiler correctness thm:
-
-    !wprog t1 t2 d1 res c.
-      ?p n.
-        state_rel p t1 d1 /\
-        colouring_ok wprog c /\ res <> SOME Error /\
-        wEval (wprog,t1) = (res,t2) ==>
-        ?d2. wEval (apply_colour c wprog,d1) = (res,d2) /\
-             state_rel (\i. p (i+n)) t2 d2
-
-    where state_rel is roughly
-
-    state_rel p t1 d1 =
-      ?dp dl dc.
-        (d1 = t1 with <| permute := dp; locals := dl; code := dc |>) /\
-        t1.permute = p /\
-        !k arity code.
-          lookup k t1.code = SOME (arity,code)
-          ?c. colouring_ok code c /\
-              lookup k d1.code = SOME (arity,apply_colour c code)
-
-  word_lang --> stack_lang compiler correctness thm:
-
-    wEval (wprog,t1 with permute := K I) = (res,t2) ==>
-    sEval (wCompile wprog,r1) = (res1,r2)
-
-*)
 val _ = export_theory();
